Add crash borrow related things

src/base/adequacy.v
@@ -34,6 +34,7 @@ Definition nvm_build_delta Σ Hc (names : nvm_base_names) : nvmBaseDeltaG Σ :=
     nvm_base_names' := names;
   |}.
 
+(* Allocate the state intepretation in the base logic for any valid heap. *)
 Lemma allocate_state_interp `{hPre : !nvmBaseGpreS Σ} Hinv Hc σ :
   valid_heap σ.1 →
   ⊢ |==> ∃ (names : nvm_base_names),
@@ -118,36 +119,37 @@ Proof.
   - done.
 Qed.
 
-(* Similar to the [reccv_adequate] in Perennial except the invariant is removed. *)
+(* Similar to the [reccv_adequate] in Perennial except that:
+   1. The invariant is removed.
+   2. We ignore the global state (which is [unit] for nvm_lang). *)
 Record recv_adequate (s : stuckness) (e1 r1: thread_state) (σ1 : state nvm_lang)
-       (g1 : global_state nvm_lang)
-       (φ φr: thread_val → state nvm_lang → global_state nvm_lang → Prop) := {
-  recv_adequate_result_normal t2 σ2 g2 v2 :
-   erased_rsteps (CS := nvm_crash_lang) r1 ([e1], (σ1,g1)) (thread_of_val v2 :: t2, (σ2,g2)) Normal →
-   φ v2 σ2 g2;
-  recv_adequate_result_crashed t2 σ2 g2 v2 :
-   erased_rsteps (CS := nvm_crash_lang) r1 ([e1], (σ1,g1)) (thread_of_val v2 :: t2, (σ2,g2)) Crashed →
-   φr v2 σ2 g2;
-  recv_adequate_not_stuck t2 σ2 g2 e2 stat :
+       (φ φr: thread_val → state nvm_lang → Prop) := {
+  recv_adequate_result_normal t2 σ2 v2 :
+   erased_rsteps (CS := nvm_crash_lang) r1 ([e1], (σ1,())) (thread_of_val v2 :: t2, (σ2,())) Normal →
+   φ v2 σ2;
+  recv_adequate_result_crashed t2 σ2 v2 :
+   erased_rsteps (CS := nvm_crash_lang) r1 ([e1], (σ1,())) (thread_of_val v2 :: t2, (σ2,())) Crashed →
+   φr v2 σ2;
+  recv_adequate_not_stuck t2 σ2 e2 stat :
    s = NotStuck →
-   erased_rsteps (CS := nvm_crash_lang) r1 ([e1], (σ1,g1)) (t2, (σ2,g2)) stat →
-   e2 ∈ t2 → (is_Some (thread_to_val e2) ∨ reducible (Λ := nvm_lang) e2 σ2 g2);
+   erased_rsteps (CS := nvm_crash_lang) r1 ([e1], (σ1,())) (t2, (σ2,())) stat →
+   e2 ∈ t2 → (is_Some (thread_to_val e2) ∨ reducible (Λ := nvm_lang) e2 σ2 ());
 }.
 
 Lemma adequacy_impl (s : stuckness) (e1 r1: thread_state) (σ1 : state nvm_lang)
-       (g1 : global_state nvm_lang)
-       (φ φr: thread_val → state nvm_lang → global_state nvm_lang → Prop) :
-  recovery_adequacy.recv_adequate (CS := nvm_crash_lang) s e1 r1 σ1 g1 φ φr (λ _ _, True) →
-  recv_adequate s e1 r1 σ1 g1 φ φr.
+       (φ φr: thread_val → state nvm_lang → Prop) :
+  recovery_adequacy.recv_adequate (CS := nvm_crash_lang)
+                                  s e1 r1 σ1 () (λ v σ _, φ v σ) (λ v σ _, φr v σ) (λ _ _, True) →
+  recv_adequate s e1 r1 σ1 φ φr.
 Proof. intros [????]. split; try naive_solver. Qed.
 
 (* This is the simpler adequacy result. *)
-Corollary base_recv_adequacy_simpl Σ `{hPre : !nvmBaseGpreS Σ} s k e r σ g φ φr :
+Corollary base_recv_adequacy_simpl Σ `{hPre : !nvmBaseGpreS Σ} s k e r σ φ φr :
   valid_heap σ.1 →
   (∀ `{Hheap : !nvmBaseFixedG Σ, hD : !nvmBaseDeltaG Σ},
     ⊢ ([∗ map] l ↦ v ∈ σ.1, l ↦h v) -∗ (
        wpr s k ⊤ e r (λ v, ⌜φ v⌝) (λ _, True) (λ _ v, ⌜φr v⌝))) →
-  recv_adequate s e r σ g (λ v _ _, φ v) (λ v _ _, φr v).
+  recv_adequate s e r σ (λ v _, φ v) (λ v _, φr v).
 Proof.
   intros val hyp.
   apply adequacy_impl.
